add 3d option --z3_produce_testcases_c, set by default

src/3d/Options.fst
@@ -34,6 +34,7 @@ let inplace_hashes : ref (list vstring) = alloc []
 let input_file : ref (list string) = alloc []
 let json : ref bool = alloc false
 let no_copy_everparse_h : ref bool = alloc false
+let no_produce_testcases_c : ref bool = alloc false
 let output_dir : ref (option vstring) = alloc None
 let save_hashes : ref bool = alloc false
 let save_z3_transcript: ref (option vstring) = alloc None
@@ -361,6 +362,7 @@ let (display_usage_2, compute_options_2, fstar_options) =
     CmdOption "z3_diff_test" (OptStringOption "parser1,parser2" valid_equate_types z3_diff_test) "produce differential tests for two parsers" [];
     CmdOption "z3_executable" (OptStringOption "path/to/z3" always_valid z3_executable) "z3 executable for test case generation (default `z3`; does not affect verification of generated F* code)" [];
     CmdOption "z3_options" (OptStringOption "'options to z3'" always_valid z3_options) "command-line options to pass to z3 for test case generation (does not affect verification of generated F* code)" [];
+    CmdOption "no_z3_produce_testcases_c" (OptBool no_produce_testcases_c) "Do not write the generated test cases to <output directory>/testcases.c" [];
     CmdOption "z3_test" (OptStringOption "parser name" always_valid z3_test) "produce positive and/or negative test cases for a given parser" [];
     CmdOption "z3_test_mode" (OptStringOption "pos|neg|all" valid_z3_test_mode z3_test_mode) "produce positive, negative, or all kinds of test cases (default all)" [];
     CmdOption "z3_witnesses" (OptStringOption "nb" always_valid z3_witnesses) "ask for nb distinct test witnesses per branch case (default 1)" [];
@@ -590,6 +592,9 @@ let get_z3_options () : ML string =
   match !z3_options with
   | None -> ""
   | Some s -> s
+
+let get_produce_testcases_c () : ML bool =
+  not !no_produce_testcases_c
 
 let get_fstar_exe () : ML string =
   match !fstar_exe with
